big semantics THETIME + THESTATE + TERMINATES

IMP-/Big_StepT.thy
@@ -1,4 +1,158 @@
 theory Big_StepT
-imports Main Com
-begin
+imports Main Com begin
+text "do we need to import Big_Step"
+inductive
+  big_step_t :: "com \<times> state \<Rightarrow> nat \<Rightarrow> state \<Rightarrow> bool"  ("_ \<Rightarrow> _ \<Down> _" 55)
+where
+Skip: "(SKIP,s) \<Rightarrow> Suc (0::nat) \<Down> s"|
+Assign: "(x ::= a,s) \<Rightarrow> Suc 0 \<Down> s(x := aval a s)" |
+Seq: "\<lbrakk> (c1,s1) \<Rightarrow> x \<Down> s2;  (c2,s2) \<Rightarrow> y \<Down> s3 ; z=x+y \<rbrakk> \<Longrightarrow> (c1;;c2, s1) \<Rightarrow> z \<Down> s3" |
+IfTrue: "\<lbrakk> s b \<noteq> 0;  (c1,s) \<Rightarrow> x \<Down> t; y=x+1 \<rbrakk> \<Longrightarrow> (IF b \<noteq>0 THEN c1 ELSE c2, s) \<Rightarrow> y \<Down> t" |
+IfFalse: "\<lbrakk> s b = 0; (c2,s) \<Rightarrow> x \<Down> t; y=x+1  \<rbrakk> \<Longrightarrow> (IF b \<noteq>0 THEN c1 ELSE c2, s) \<Rightarrow> y \<Down> t" |
+WhileFalse: "\<lbrakk> s b = 0 \<rbrakk> \<Longrightarrow> (WHILE b \<noteq>0 DO c,s) \<Rightarrow> Suc 0 \<Down> s" |
+WhileTrue: "\<lbrakk> s1 b \<noteq> 0;  (c,s1) \<Rightarrow> x \<Down> s2;  (WHILE b \<noteq>0 DO c, s2) \<Rightarrow> y \<Down> s3; 1+x+y=z  \<rbrakk> 
+    \<Longrightarrow> (WHILE b \<noteq>0 DO c, s1) \<Rightarrow> z \<Down> s3" 
+code_pred big_step_t .
+
+schematic_goal ex: "(''x'' ::= A (N 5);; ''y'' ::= A (V ''x''), s) \<Rightarrow> ?t \<Down> ?s"
+apply(rule Seq)
+apply(rule Assign)
+apply simp
+apply(rule Assign)
+apply simp
+done
+thm ex[simplified]
+
+
+values "{(t, x). big_step_t (SKIP, \<lambda>_. 0) x t}"
+
+values "{map t [''x''] |t x. (SKIP, <''x'' := 42>) \<Rightarrow> x \<Down> t}"
+
+values "{map t [''x''] |t x. (''x'' ::=A (N 2), <''x'' := 42>) \<Rightarrow> x \<Down> t}"
+
+values "{(map t [''x''],x) |t x. (WHILE ''x''\<noteq>0 DO ''x''::= Sub (V ''x'') (N 1),<''x'':=5>) \<Rightarrow> x \<Down> t }"
+
+text "what does it mean exactly ?"
+declare big_step_t.intros [intro]
+
+lemmas big_step_t_induct = big_step_t.induct[split_format(complete)]
+
+inductive_cases Skip_tE[elim!]: "(SKIP,s) \<Rightarrow> x \<Down> t"
+thm Skip_tE
+inductive_cases Assign_tE[elim!]: "(x ::= a,s) \<Rightarrow> p \<Down> t"
+thm Assign_tE
+inductive_cases Seq_tE[elim!]: "(c1;;c2,s1) \<Rightarrow> p \<Down> s3"
+thm Seq_tE
+inductive_cases If_tE[elim!]: "(IF b \<noteq>0 THEN c1 ELSE c2,s) \<Rightarrow> x \<Down> t"
+thm If_tE
+
+inductive_cases While_tE[elim]: "(WHILE b \<noteq>0 DO c,s) \<Rightarrow> x \<Down> t"
+thm While_tE
+
+lemma "(IF b \<noteq>0 THEN SKIP ELSE SKIP, s) \<Rightarrow> x \<Down> t \<Longrightarrow> t = s"
+  by blast
+
+lemma assumes "(IF b \<noteq>0 THEN SKIP ELSE SKIP, s) \<Rightarrow> x \<Down> t"
+  shows "t = s"
+proof -
+  from assms show ?thesis
+  proof cases
+  case (IfTrue x)
+  then show ?thesis by blast
+next
+  case (IfFalse x)
+  then show ?thesis by blast
+qed
+qed
+lemma assign_t_simp:
+  "((x ::= a,s) \<Rightarrow> Suc 0 \<Down>  s') \<longleftrightarrow> (s' = s(x := aval a s))"
+  by (auto)
+
+text "goal_cases"
+text "delete  \<noteq> ==> 0< from simp"
+theorem big_step_t_determ2: "\<lbrakk> (c,s) \<Rightarrow> p \<Down> t; (c,s) \<Rightarrow> q \<Down> u \<rbrakk> \<Longrightarrow> (u = t \<and> p=q)"
+  apply  (induction arbitrary: u q rule: big_step_t_induct)
+    apply(elim Skip_tE) apply(simp)
+    apply(elim Assign_tE) apply(simp)
+  apply blast
+    apply(elim If_tE) apply(simp) apply blast
+    apply(elim If_tE)  apply (linarith)apply simp
+    apply(erule While_tE) apply(simp) apply simp
+    proof (goal_cases)
+      case 1
+      from 1(7) show ?case apply(safe) 
+        apply(erule While_tE)
+          using 1(1-6) apply fast
+          using 1(1-6) apply (simp)
+        apply(erule While_tE)
+          using 1(1-6) apply fast
+          using 1(1-6) by (simp)
+      qed
+
+lemma bigstep_det: "(c1, s) \<Rightarrow> p1 \<Down> t1 \<Longrightarrow> (c1, s) \<Rightarrow> p \<Down> t \<Longrightarrow> p1=p \<and> t1=t"
+  using big_step_t_determ2 by simp
+lemma bigstep_progress: "(c, s) \<Rightarrow> p \<Down> t \<Longrightarrow> p > 0"
+  apply(induct rule: big_step_t.induct, auto) done
+
+abbreviation terminates ("\<down>") where "terminates cs \<equiv> (\<exists>n a. (cs \<Rightarrow> n \<Down> a))"
+abbreviation thestate ("\<down>\<^sub>s") where "thestate cs \<equiv> (THE a. \<exists>n. (cs \<Rightarrow> n \<Down> a))" 
+abbreviation thetime ("\<down>\<^sub>t") where "thetime cs \<equiv> (THE n. \<exists>a. (cs \<Rightarrow> n \<Down> a))"
+
+lemma bigstepT_the_cost: "(c, s) \<Rightarrow> t \<Down> s' \<Longrightarrow> \<down>\<^sub>t(c, s) = t"
+  using bigstep_det by blast 
+
+lemma bigstepT_the_state: "(c, s) \<Rightarrow> t \<Down> s' \<Longrightarrow> \<down>\<^sub>s(c, s) = s'"
+  using bigstep_det by blast 
+
+lemma SKIPnot: "(\<not> (SKIP, s) \<Rightarrow> p \<Down> t) \<longleftrightarrow> (s\<noteq>t \<or> p\<noteq>Suc 0)" by blast
+
+lemma SKIPp: "\<down>\<^sub>t(SKIP,s) = Suc 0"
+  apply(rule the_equality)
+  apply fast
+  apply auto done 
+
+lemma SKIPt: "\<down>\<^sub>s(SKIP,s) = s"
+  apply(rule the_equality)
+  apply fast
+  apply auto done 
+
+
+lemma ASSp: "(THE p. Ex (big_step_t (x ::= e, s) p)) = Suc 0"
+  apply(rule the_equality)
+  apply fast
+  apply auto done 
+
+lemma ASSt: "(THE t. \<exists>p. (x ::= e, s) \<Rightarrow> p \<Down> t) = s(x := aval e s)"
+  apply(rule the_equality)
+  apply fast
+  apply auto done 
+
+lemma ASSnot: "( \<not> (x ::= e, s) \<Rightarrow> p \<Down> t ) = (p\<noteq>Suc 0 \<or> t\<noteq>s(x := aval e s))"
+  apply auto done
+
+lemma If_THE_True: "Suc (THE n. \<exists>a. (c1, s) \<Rightarrow> n \<Down> a) =  (THE n. \<exists>a. (IF b \<noteq>0 THEN c1 ELSE c2, s) \<Rightarrow> n \<Down> a)"
+     if T: "s b \<noteq> 0" and c1_t: "terminates (c1,s)" for s l
+proof -
+  from c1_t obtain p t where a: "(c1, s) \<Rightarrow> p \<Down> t" by blast
+  with T have b: "(IF b \<noteq>0 THEN c1 ELSE c2, s) \<Rightarrow> p+1 \<Down> t"  using IfTrue by simp
+  from a bigstepT_the_cost have "(THE n. \<exists>a. (c1, s) \<Rightarrow> n \<Down> a) = p" by simp
+moreover    
+  from b bigstepT_the_cost have "(THE n. \<exists>a. (IF b \<noteq>0 THEN c1 ELSE c2, s) \<Rightarrow> n \<Down> a) = p+1" by simp
+ultimately
+  show ?thesis by simp
+qed
+
+lemma If_THE_False: "Suc (THE n. \<exists>a. (c2, s) \<Rightarrow> n \<Down> a) =  (THE n. \<exists>a. (IF b \<noteq>0 THEN c1 ELSE c2, s) \<Rightarrow> n \<Down> a)"
+     if T: "s b = 0" and c2_t: "\<down> (c2,s)" for s l
+proof -
+  from c2_t obtain p t where a: "(c2, s) \<Rightarrow> p \<Down> t"  by blast
+  with T have b: "(IF b \<noteq>0 THEN c1 ELSE c2, s) \<Rightarrow> p+1 \<Down> t"  using IfFalse by simp
+  from a bigstepT_the_cost have "(THE n. \<exists>a. (c2, s) \<Rightarrow> n \<Down> a) = p" by simp
+moreover    
+  from b bigstepT_the_cost have "(THE n. \<exists>a. (IF b \<noteq>0 THEN c1 ELSE c2, s) \<Rightarrow> n \<Down> a) = p+1" by simp
+ultimately
+  show ?thesis by simp
+qed
+    
+
 end
